theories/AlgorithmicTyping.v
@@ -1,7 +1,6 @@
 (** * LogRel.AlgorithmicTyping: definition of algorithmic conversion and typing. *)
 From Coq Require Import ssrbool.
-From LogRel.AutoSubst Require Import core unscoped Ast Extra.
-From LogRel Require Import Utils BasicAst Notations Context NormalForms Weakening UntypedReduction GenericTyping.
+From LogRel Require Import Utils Syntax.All GenericTyping.
 
 Section Definitions.
 
